Clean up calculation and display of statistics

src/StandardLibrary.dfy
@@ -93,4 +93,39 @@ module StandardLibrary {
   {
     resultSeq := SetToSeq(m.Items);
   }
+
+  function method MinReal(a: real, b: real): real
+  {
+    if a < b
+      then a
+    else
+      b
+  }
+
+  function method MaxReal(a: real, b: real): real
+  {
+    if a < b
+      then b
+    else
+      a
+  }
+
+  function method {:opaque} MinRealSeq(s: seq<real>): real
+    requires 0 < |s|
+    ensures forall k {:trigger k in s} :: k in s ==> MinRealSeq(s) <= k
+    ensures MinRealSeq(s) in s
+  {
+    assert s == [s[0]] + s[1..];
+    if |s| == 1 then s[0] else MinReal(s[0], MinRealSeq(s[1..]))
+  }
+
+  function method {:opaque} MaxRealSeq(s: seq<real>): real
+    requires 0 < |s|
+    ensures forall k {:trigger k in s} :: k in s ==> k <= MaxRealSeq(s)
+    ensures MaxRealSeq(s) in s
+  {
+    assert s == [s[0]] + s[1..];
+    if |s| == 1 then s[0] else MaxReal(s[0], MaxRealSeq(s[1..]))
+  }
+
 }
